serializing a timestamp as an iv

steel/Zeta.Steel.LogEntry.Spec.fsti
@@ -89,7 +89,17 @@ val spec_parser_u256_never_fails (b:Seq.seq U8.t { Seq.length b == 32 })
            | None -> False
            | Some (_, n) -> n == 32)
 
-val spec_parser_iv : spec_parser timestamp
-val spec_serializer_iv: spec_serializer spec_parser_iv
-val serialized_iv_length (s:timestamp)
-  : Lemma (Seq.length (spec_serializer_iv s) == 96)
+
+val spec_parser_timestamp : spec_parser timestamp
+val spec_serialize_timestamp : spec_serializer spec_parser_timestamp
+val serialized_timestamp_length (ts:timestamp)
+  : Lemma (Seq.length (spec_serialize_timestamp ts) == 8)
+          [SMTPat (Seq.length (spec_serialize_timestamp ts))]
+
+let spec_serialize_iv (ts:timestamp) = 
+  Seq.append (spec_serialize_timestamp ts)
+             (Seq.create 88 0uy)
+
+let serialized_iv_length (s:timestamp)
+  : Lemma (Seq.length (spec_serialize_iv s) == 96)
+  = ()
