steel/Zeta.Steel.LogEntry.fsti
@@ -29,7 +29,7 @@ inline_for_extraction
 noextract
 let parser_u256 : parser spec_parser_u256 = zeta__parser_u256
 
-val zeta__serialize_iv : serializer spec_serializer_iv
+val zeta__serialize_timestamp : serializer spec_serialize_timestamp
 
 noextract
 let timestamp_len = 8
@@ -42,6 +42,28 @@ let seq_suffix_is_zero (s:Seq.seq byte)
 
 module A = Steel.ST.Array
 open Steel.ST.Util
+let serialize_timestamp (#bs:Ghost.erased (Seq.seq FStar.UInt8.t))
+                        (a:byte_array { A.length a == 8 })
+                        (v: timestamp)
+ : STT U32.t
+    (A.pts_to a full_perm bs)
+    (fun slice_len ->
+       exists_ (fun (bs:_) ->
+         A.pts_to a full_perm bs `star`
+         pure (
+           spec_serialize_timestamp v == bs)))
+ = admit_(); return 0ul
+
+let seq_suffix_is_zero_elim (s:Seq.seq byte)
+                            (from:nat)
+  : Lemma 
+    (requires seq_suffix_is_zero s from)
+    (ensures
+         from <= Seq.length s /\
+         Seq.slice s from (Seq.length s) `Seq.equal` Seq.create (Seq.length s - from) 0uy)
+  = ()
+
+
 let serialize_iv (a:byte_array { A.length a == 96 })
                  (v: timestamp)
   : Steel.ST.Util.STT unit
@@ -51,5 +73,21 @@ let serialize_iv (a:byte_array { A.length a == 96 })
          A.pts_to a full_perm bs `star`
          pure (
            seq_suffix_is_zero bs timestamp_len /\
-           spec_serializer_iv v == bs)))
-  = admit_()
+           spec_serialize_iv v == bs)))
+  = let bs = elim_exists () in
+    A.pts_to_length a bs;
+    elim_pure _;
+    seq_suffix_is_zero_elim bs timestamp_len;
+    let adj = A.ghost_split a 8sz in
+    let n = serialize_timestamp (A.split_l a 8sz) v in 
+    let bs_l = elim_exists () in
+    A.pts_to_length (A.split_l a 8sz) bs_l;
+    elim_pure _;
+    assert_ (A.pts_to (A.split_l a 8sz) full_perm bs_l `star`
+             A.pts_to (A.split_r a 8sz) full_perm (Seq.slice bs 8 (Seq.length bs)));
+    A.ghost_join (A.split_l a 8sz) (A.split_r a 8sz) adj;
+    rewrite (A.pts_to (A.merge (A.split_l a 8sz) (A.split_r a 8sz)) _ _)
+            (A.pts_to a full_perm (spec_serialize_iv v));
+    intro_pure (seq_suffix_is_zero (spec_serialize_iv v) timestamp_len /\
+                spec_serialize_iv v == spec_serialize_iv v);
+    return ()
